\documentclass{article}
\topmargin = 0in
\oddsidemargin = 0in
\evensidemargin = \oddsidemargin
\textwidth = 6.5in
\textheight = 8in
\usepackage{times}
\usepackage{bcprules}
\usepackage{amsthm}
\usepackage{syntax}
\usepackage{trfrac}
\usepackage{mathtools}

\renewcommand{\syntleft}{\normalfont\itshape}
\renewcommand{\syntright}{}

\newcommand{\step}[2]{{\tt #1} $\longrightarrow$ {\tt #2}}
\newcommand{\eval}[2]{{\tt #1} $\Downarrow$ {\tt #2}}
\newcommand{\tc}[3]{{\tt #1} $\vdash$ {\tt #2} \ : \ {\tt #3}}
\newcommand{\tcDef}[2]{{\tt #1}\ : \ {\tt #2}}

\newcommand{\inferrule}[3]{\infrule[#1]{\mbox{#2}}{\mbox{#3}}}
\newcommand{\inferax}[2]{\infrule[#1]{\mbox{}}{\mbox{#2}}}

\newcommand{\term}[1]{{\tt t$_{#1}$}}
\newcommand{\mathType}[2]{\mathtt{#1}:\mathtt{#2}}
\newcommand{\iftt}[3]{\mathtt{if}\ #1\ \mathtt{then}\ #2\ \mathtt{else}\ #3}


\title{Homework 4}

\author{Eric Marcin-Cuddy and John Bender, CS 231}

\date{November 19th, 2013}

\begin{document}

\maketitle

\begin{enumerate}
  \item \texttt{while} loop
    \begin{enumerate}
      \item Operational Semantics
        \begin{equation*}
          \trfrac[E-While]{}{
            \mathtt{while}\  t_1\ \mathtt{do}\ t_2 \rightarrow
            \iftt{t_1}{t_2;(\mathtt{while}\  t_1\ \mathtt{do}\ t_2)}{\mathtt{unit}}
          }
        \end{equation*}

      \item Type Rule
        \begin{equation*}
          \trfrac[T-While]{
            \Gamma \vdash t_1 : \mathtt{Bool} \qquad \Gamma \vdash t_2 : \mathtt{Unit}
          }{
            \Gamma \vdash \mathtt{while}\  t_1\ \mathtt{do}\ t_2 : \mathtt{Unit}
          }
        \end{equation*}
      \item \texttt{whileFun}
        \begin{align*}
          & \mathtt{let\ rec\ whileFun} =\\
          &\qquad \lambda x\mathtt{:Unit}.\iftt{t_1}{(\mathtt{whileFun}\ t_2);\ x}{\mathtt{unit}}
        \end{align*}

      \item \texttt{whileFun2}
        \begin{align*}
          & \mathtt{let\ rec\ whileFun2} =\\
          &\qquad \lambda t_1\mathtt{:Bool}.
            \lambda t_2\mathtt{:Unit}.
            \iftt{t_1}{(\mathtt{whileFun2}\; t_1\; t_2);\ t_2}{\mathtt{unit}}
        \end{align*}

        \begin{align*}
          \mathtt{whileFun2}\;t_1\;t_2
        \end{align*}
    \end{enumerate}
  \item Type Inference
    \begin{enumerate}
      \item Derivation
        \begin{align*}
          & \Gamma = \emptyset, x:X, y:Y, z:Z \\
          & \Phi = \{X = Z \rightarrow M\} \cup \{Y = Z \rightarrow N\} \cup \{M = N \rightarrow O\} \\
          & \trfrac[CT-Abs]{
            \trfrac[CT-Abs]{
              \trfrac[CT-Abs]{
                \trfrac[CT-Abs]{
                  \trfrac[CT-App]{
                    \trfrac[CT-Var]{
                      x : X \in \Gamma
                    }{
                      \Gamma \vdash x : X\ |\ \{\}
                    }
                    \qquad
                    \trfrac[CT-Var]{
                      z : Z \in \Gamma
                    }{
                      \Gamma \vdash z : Z\ |\ \{\}
                    }
                  }{
                    \Gamma \vdash (x\ z) : M \ |\ \{\} \cup \{\} \cup \{X = Z \rightarrow M\}
                  }
                  \qquad
                  \trfrac[CT-App]{
                    \trfrac[CT-Var]{
                      y : Y \in \Gamma
                    }{
                      \Gamma \vdash y : Y\ |\ \{\}
                    }
                    \qquad
                    \trfrac[CT-Var]{
                      z : Z \in \Gamma
                    }{
                      \Gamma \vdash z : Z\ |\ \{\}
                    }
                  }{
                    \Gamma \vdash (y\ z) : N \ |\ \{\} \cup \{\} \cup \{Y = Z \rightarrow N\}
                  }
                }{
                  \Gamma \vdash (x\ z)\ (y\ z) : O\ |\ \Phi
                }
              }{
                \emptyset, x:X, y:Y \vdash \lambda z:Z.((x\ z)\ (y\ z)) : Z \rightarrow O \ |\ \Phi
              }
            }{
              \emptyset, x:X \vdash \lambda y:Y.\lambda z:Z.((x\ z)\ (y\ z)) : Y \rightarrow (Z \rightarrow O)\ |\ \Phi
            }
          }{
            \emptyset \vdash \lambda x:X.\lambda y:Y.\lambda z:Z.((x\ z)\ (y\ z)) : X \rightarrow (Y \rightarrow (Z \rightarrow O))\ |\ \Phi
          }
        \end{align*}

        \item Substitution
          \begin{align*}
            & \sigma = \lambda t.[Z \mapsto P][Y \mapsto (P \rightarrow N)][X \mapsto (P \rightarrow (N \rightarrow O))]t \\ \\
            & \sigma(X \rightarrow (Y \rightarrow (Z \rightarrow O))) = \\
            & \qquad (P \rightarrow (N \rightarrow O)) \rightarrow ((P \rightarrow N) \rightarrow (P \rightarrow O)) \\ \\
            & \sigma(\lambda x:X.\lambda y:Y.\lambda z:Z.((x\ z)\ (y\ z)) = \\
            & \qquad \lambda x:(P \rightarrow (N \rightarrow O)).
                     \lambda y:(P \rightarrow N).
                     \lambda z:P.((x\ z)\ (y\ z)
          \end{align*}
        \end{enumerate}
  \end{enumerate}

\end{document}
